BB_sem_asgn_equiv.v
@@ -29,6 +29,7 @@ Lemma Q_asgn:
 Proof.
   intros. unfold Qb. left.  rename H0 into BBnownum_prop. rename H into jmp_prop. rename H1 into BBnow_not_jmp_toself.
   rename H2 into jmp_condition. 
+  split. unfold is_asgn. simpl. reflexivity.
   exists {|
     block_num := BBnow.(block_num);
     commands := BBnow.(cmd) ++ {| X:= x; E:= e|} :: nil;
